Phi_Semantics/PhiSem_Common_Int.thy
@@ -146,7 +146,7 @@ lemma synthesis_const_by_imp:
   \<open> R \<t>\<r>\<a>\<n>\<s>\<f>\<o>\<r>\<m>\<s> const \<Ztypecolon> \<v>\<a>\<l>[\<phi>literal v] T \<r>\<e>\<m>\<a>\<i>\<n>\<s> R @action synthesis
 \<Longrightarrow> \<p>\<r>\<o>\<c> Return (\<phi>literal v) \<lbrace> R \<longmapsto> \<lambda>ret. const \<Ztypecolon> \<v>\<a>\<l>[ret] T \<r>\<e>\<m>\<a>\<i>\<n>\<s> R \<rbrace> @action synthesis\<close>
   unfolding Action_Tag_def Premise_def \<phi>Procedure_def det_lift_def Return_def \<phi>literal_def Transformation_def
-  apply (clarsimp simp add: Val.unfold INTERP_SPEC_subj Subjection_expn_set INTERP_SPEC)
+  by (clarsimp simp add: Val.unfold INTERP_SPEC_subj Subjection_expn_set INTERP_SPEC)
 
 
 (*lemma make_synthesis_rule_for_const:
@@ -205,19 +205,19 @@ lemmas [\<phi>reason 2010 for \<open>PROP Gen_Synthesis_Rule (
 *)
 
 lemma [\<phi>reason 200]:
-  \<open> \<p>\<r>\<o>\<c> H \<lbrace> R1 \<longmapsto> \<lambda>ret. R2\<heavy_comma> \<blangle> 1 \<Ztypecolon> T ret \<brangle> \<rbrace> \<t>\<h>\<r>\<o>\<w>\<s> E @action synthesis
-\<Longrightarrow> \<p>\<r>\<o>\<c> H \<lbrace> R1 \<longmapsto> \<lambda>ret. R2\<heavy_comma> \<blangle> Suc 0 \<Ztypecolon> T ret \<brangle> \<rbrace> \<t>\<h>\<r>\<o>\<w>\<s> E @action synthesis\<close>
+  \<open> \<p>\<r>\<o>\<c> H \<lbrace> R1 \<longmapsto> \<lambda>ret. 1 \<Ztypecolon> T ret \<r>\<e>\<m>\<a>\<i>\<n>\<s> R2 \<rbrace> \<t>\<h>\<r>\<o>\<w>\<s> E @action synthesis
+\<Longrightarrow> \<p>\<r>\<o>\<c> H \<lbrace> R1 \<longmapsto> \<lambda>ret. Suc 0 \<Ztypecolon> T ret \<r>\<e>\<m>\<a>\<i>\<n>\<s> R2 \<rbrace> \<t>\<h>\<r>\<o>\<w>\<s> E @action synthesis\<close>
   unfolding One_nat_def .
 
 lemma [\<phi>reason 200]:
-  \<open> \<p>\<r>\<o>\<c> f \<lbrace> X \<longmapsto> \<lambda>ret. R\<heavy_comma> \<blangle> push_bit n x \<Ztypecolon> Y ret \<brangle> \<rbrace> \<t>\<h>\<r>\<o>\<w>\<s> E @action synthesis
-\<Longrightarrow> \<p>\<r>\<o>\<c> f \<lbrace> X \<longmapsto> \<lambda>ret. R\<heavy_comma> \<blangle> x * 2 ^ n \<Ztypecolon> Y ret \<brangle> \<rbrace> \<t>\<h>\<r>\<o>\<w>\<s> E @action synthesis\<close>
+  \<open> \<p>\<r>\<o>\<c> f \<lbrace> X \<longmapsto> \<lambda>ret. push_bit n x \<Ztypecolon> Y ret \<r>\<e>\<m>\<a>\<i>\<n>\<s> R \<rbrace> \<t>\<h>\<r>\<o>\<w>\<s> E @action synthesis
+\<Longrightarrow> \<p>\<r>\<o>\<c> f \<lbrace> X \<longmapsto> \<lambda>ret. x * 2 ^ n \<Ztypecolon> Y ret \<r>\<e>\<m>\<a>\<i>\<n>\<s> R \<rbrace> \<t>\<h>\<r>\<o>\<w>\<s> E @action synthesis\<close>
   for x :: nat
   unfolding push_bit_nat_def .
 
 lemma [\<phi>reason 200]:
-  \<open> \<p>\<r>\<o>\<c> f \<lbrace> X \<longmapsto> \<lambda>ret. R\<heavy_comma> \<blangle> push_bit n x \<Ztypecolon> Y ret \<brangle> \<rbrace> \<t>\<h>\<r>\<o>\<w>\<s> E @action synthesis
-\<Longrightarrow> \<p>\<r>\<o>\<c> f \<lbrace> X \<longmapsto> \<lambda>ret. R\<heavy_comma> \<blangle> x * 2 ^ n \<Ztypecolon> Y ret \<brangle> \<rbrace> \<t>\<h>\<r>\<o>\<w>\<s> E @action synthesis\<close>
+  \<open> \<p>\<r>\<o>\<c> f \<lbrace> X \<longmapsto> \<lambda>ret. push_bit n x \<Ztypecolon> Y ret \<r>\<e>\<m>\<a>\<i>\<n>\<s> R \<rbrace> \<t>\<h>\<r>\<o>\<w>\<s> E @action synthesis
+\<Longrightarrow> \<p>\<r>\<o>\<c> f \<lbrace> X \<longmapsto> \<lambda>ret. x * 2 ^ n \<Ztypecolon> Y ret \<r>\<e>\<m>\<a>\<i>\<n>\<s> R \<rbrace> \<t>\<h>\<r>\<o>\<w>\<s> E @action synthesis\<close>
   for x :: int
   unfolding push_bit_int_def .
 
